code/bignum/Hacl.Spec.Bignum.ExpFW.fst
@@ -9,6 +9,7 @@ open Hacl.Spec.Bignum.Definitions
 
 module Loops = Lib.LoopCombinators
 module LSeq = Lib.Sequence
+module LE  = Lib.Exponentiation
 
 module E = Hacl.Spec.Exponentiation.Lemmas
 module M = Hacl.Spec.Montgomery.Lemmas
@@ -99,6 +100,26 @@ let table_select_ct #t #nLen table_len table i =
   Loops.repeati (table_len - 1) (table_select_ct_f #t #nLen table_len table i) res0
 
 
+val bn_get_bits_l:
+    #t:limb_t
+  -> bBits:size_pos
+  -> bLen:size_nat{bLen == blocks bBits (bits t)}
+  -> b:lbignum t bLen
+  -> l:size_pos{l < bits t}
+  -> i:nat{i < bBits / l} ->
+  res:limb t{v res < pow2 l}
+
+let bn_get_bits_l #t bBits bLen b l i =
+  Math.Lemmas.lemma_mult_le_left l (i + 1) (bBits / l);
+  assert (l * (i + 1) <= l * (bBits / l));
+  Math.Lemmas.multiply_fractions bBits l;
+  assert (l * (i + 1) <= bBits);
+  let bits_l = BN.bn_get_bits b (bBits - l * i - l) l in
+  BN.bn_get_bits_lemma b (bBits - l * i - l) l;
+  assert (v bits_l < pow2 l);
+  bits_l
+
+
 val bn_mod_exp_fw_mont_f:
     #t:limb_t
   -> #nLen:size_pos
@@ -110,16 +131,13 @@ val bn_mod_exp_fw_mont_f:
   -> l:size_pos{l < bits t}
   -> table_len:size_nat{1 < table_len /\ table_len * nLen <= max_size_t /\ table_len == pow2 l}
   -> table:lbignum t (table_len * nLen)
-  -> i:nat{l * (i + 1) <= bBits}
+  -> i:nat{i < bBits / l}
   -> accM:lbignum t nLen ->
   lbignum t nLen
 
 let bn_mod_exp_fw_mont_f #t #nLen n mu bBits bLen b l table_len table i accM =
   let acc_pow2l = bn_mod_exp_pow2_mont n mu accM l in
-
-  let bits_l = BN.bn_get_bits b (bBits - l * i - l) l in
-  BN.bn_get_bits_lemma b (bBits - l * i - l) l;
-  assert (v bits_l < table_len);
+  let bits_l = bn_get_bits_l bBits bLen b l i in
 
   Math.Lemmas.lemma_mult_le_right nLen (v bits_l + 1) table_len;
   let a_powbits_l = sub table (v bits_l * nLen) nLen in
@@ -215,6 +233,100 @@ let rec bn_mod_exp_pow2_mont_lemma #t #nLen n mu aM b =
     () end
 
 
+val bn_mod_precomp_table_mont_f_lemma:
+    #t:limb_t
+  -> #nLen:size_pos
+  -> n:lbignum t nLen
+  -> mu:limb t
+  -> aM:lbignum t nLen
+  -> table_len:size_nat{1 < table_len /\ table_len * nLen <= max_size_t}
+  -> i:nat{i < table_len - 2}
+  -> table:lbignum t (table_len * nLen)
+  -> j:nat{j <= i + 1} ->
+  Lemma (
+    let res = bn_mod_precomp_table_mont_f n mu aM table_len i table in
+    sub res (j * nLen) nLen == sub table (j * nLen) nLen)
+
+let bn_mod_precomp_table_mont_f_lemma #t #nLen n mu aM table_len i table j =
+  Math.Lemmas.lemma_mult_le_right nLen (i + 3) table_len;
+  let t1 = sub table ((i + 1) * nLen) nLen in
+  let r = BM.bn_mont_mul n mu t1 aM in
+  let res = update_sub table ((i + 2) * nLen) nLen r in
+
+  Math.Lemmas.lemma_mult_le_right nLen (j + 1) table_len;
+  let aux (l:nat{l < nLen}) : Lemma (index (sub res (j * nLen) nLen) l == index (sub table (j * nLen) nLen) l) =
+    Math.Lemmas.lemma_mult_le_right nLen (j + 1) (i + 2);
+    assert (j * nLen + l < (i + 2) * nLen);
+    Seq.lemma_index_slice res (j * nLen) (j * nLen + nLen) l;
+    Seq.lemma_index_slice table (j * nLen) (j * nLen + nLen) l;
+    assert (index res (j * nLen + l) == index table (j * nLen + l));
+    () in
+
+  Classical.forall_intro aux;
+  LSeq.eq_intro (sub res (j * nLen) nLen) (sub table (j * nLen) nLen)
+
+
+val bn_mod_precomp_table_mont_map:
+    #t:limb_t
+  -> #nLen:size_pos
+  -> n:lbignum t nLen
+  -> table_len:size_nat{1 < table_len /\ table_len * nLen <= max_size_t}
+  -> t01:lbignum t (table_len * nLen)
+  -> t02:lseq nat table_len
+  -> j:nat{j < table_len} ->
+  Type0
+
+let bn_mod_precomp_table_mont_map #t #nLen n table_len t01 t02 j =
+  Math.Lemmas.lemma_mult_le_right nLen (j + 1) table_len;
+  let bj = sub t01 (j * nLen) nLen in
+  bn_v bj == index t02 j /\ bn_v bj < bn_v n
+
+
+val bn_mod_precomp_table_mont_step_lemma:
+    #t:limb_t
+  -> #nLen:size_pos
+  -> n:lbignum t nLen
+  -> mu:limb t
+  -> aM:lbignum t nLen
+  -> table_len:size_nat{1 < table_len /\ table_len * nLen <= max_size_t}
+  -> i:nat{i < table_len - 2}
+  -> t01:lbignum t (table_len * nLen)
+  -> t02:lseq nat table_len ->
+  Lemma
+  (requires
+    BM.bn_mont_pre n mu /\ bn_v aM < bn_v n /\
+    (forall (j:nat{j <= i + 1}). {:pattern bn_mod_precomp_table_mont_map n table_len t01 t02 j}
+      bn_mod_precomp_table_mont_map n table_len t01 t02 j))
+  (ensures
+    (let t3: lbignum t (table_len * nLen) = bn_mod_precomp_table_mont_f n mu aM table_len i t01 in
+     let t4: lseq nat table_len = E.mod_precomp_table_mont_f (bits t) nLen (bn_v n) (v mu) (bn_v aM) table_len i t02 in
+     (forall (j:nat{j <= i + 2}). {:pattern bn_mod_precomp_table_mont_map n table_len t3 t4 j}
+       bn_mod_precomp_table_mont_map n table_len t3 t4 j)))
+
+let bn_mod_precomp_table_mont_step_lemma #t #nLen n mu aM table_len i t01 t02 =
+  let t3: lbignum t (table_len * nLen) = bn_mod_precomp_table_mont_f n mu aM table_len i t01 in
+  let t4: lseq nat table_len = E.mod_precomp_table_mont_f (bits t) nLen (bn_v n) (v mu) (bn_v aM) table_len i t02 in
+  Math.Lemmas.lemma_mult_le_right nLen (i + 3) table_len;
+  assert (sub t3 ((i + 2) * nLen) nLen == BM.bn_mont_mul n mu (sub t01 ((i + 1) * nLen) nLen) aM);
+  assert (bn_mod_precomp_table_mont_map n table_len t01 t02 (i + 1));
+  BM.bn_mont_mul_lemma n mu (sub t01 ((i + 1) * nLen) nLen) aM;
+  assert (index t4 (i + 2) == M.mont_mul (bits t) nLen (bn_v n) (v mu) (index t02 (i + 1)) (bn_v aM));
+  assert (bn_mod_precomp_table_mont_map n table_len t3 t4 (i + 2));
+
+  let aux (j:nat{j <= i + 1}) : Lemma (bn_mod_precomp_table_mont_map n table_len t3 t4 j) =
+    Math.Lemmas.lemma_mult_le_right nLen (j + 1) table_len;
+    assert (index t4 j == index t02 j);
+
+    assert (bn_mod_precomp_table_mont_map n table_len t01 t02 j);
+    assert (bn_v (sub t01 (j * nLen) nLen) == index t02 j);
+    bn_mod_precomp_table_mont_f_lemma n mu aM table_len i t01 j;
+    assert (bn_v (sub t3 (j * nLen) nLen) == index t4 j);
+    assert (bn_mod_precomp_table_mont_map n table_len t3 t4 j);
+    () in
+
+  Classical.forall_intro aux
+
+
 val bn_mod_precomp_table_mont_loop_lemma:
     #t:limb_t
   -> #nLen:size_pos
@@ -227,44 +339,38 @@ val bn_mod_precomp_table_mont_loop_lemma:
   -> j:nat{j <= table_len - 2} -> Lemma
   (requires
     BM.bn_mont_pre n mu /\ bn_v aM < bn_v n /\
-    index t02 0 == bn_v (sub t01 0 nLen) /\
-    index t02 1 == bn_v (sub t01 nLen nLen))
+    index t02 0 == bn_v (sub t01 0 nLen) /\ index t02 0 < bn_v n /\
+    index t02 1 == bn_v (sub t01 nLen nLen) /\ index t02 1 < bn_v n)
   (ensures
-   (let t1: lbignum t (table_len * nLen) = Loops.repeati j (bn_mod_precomp_table_mont_f n mu aM table_len) t01 in
-    let t2: lseq nat table_len = Loops.repeati j (E.mod_precomp_table_mont_f (bits t) nLen (bn_v n) (v mu) (bn_v aM) table_len) t02 in
-    (forall (i:nat{i < j + 2}).
-     (Math.Lemmas.lemma_mult_le_right nLen (i + 1) table_len;
-      assert (i * nLen + nLen <= table_len * nLen);
-      let bi = sub t1 (i * nLen) nLen in bn_v bi == index t2 i))))
+   (let t1 = Loops.repeati j (bn_mod_precomp_table_mont_f n mu aM table_len) t01 in
+    let t2 = Loops.repeati j (E.mod_precomp_table_mont_f (bits t) nLen (bn_v n) (v mu) (bn_v aM) table_len) t02 in
+    (forall (i:nat{i < j + 2}). {:pattern bn_mod_precomp_table_mont_map n table_len t1 t2 i }
+      bn_mod_precomp_table_mont_map n table_len t1 t2 i)))
 
-let bn_mod_precomp_table_mont_loop_lemma #t #nLen n mu table_len aM t01 t02 j = admit()
-  // let t1: lbignum t (table_len * nLen) = Loops.repeati j (bn_mod_precomp_table_mont_f n mu aM table_len) t01 in
-  // let t2: lseq nat table_len = Loops.repeati j (E.mod_precomp_table_mont_f (bits t) nLen (bn_v n) (v mu) (bn_v aM) table_len) t02 in
+let rec bn_mod_precomp_table_mont_loop_lemma #t #nLen n mu table_len aM t01 t02 j =
+  let t1 = Loops.repeati j (bn_mod_precomp_table_mont_f n mu aM table_len) t01 in
+  let t2 = Loops.repeati j (E.mod_precomp_table_mont_f (bits t) nLen (bn_v n) (v mu) (bn_v aM) table_len) t02 in
 
-  // if j = 0 then begin
-  //   Loops.eq_repeati0 j (bn_mod_precomp_table_mont_f n mu aM table_len) t01;
-  //   Loops.eq_repeati0 j (E.mod_precomp_table_mont_f (bits t) nLen (bn_v n) (v mu) (bn_v aM) table_len) t02;
-  //   () end
-  // else begin
-  //   let t3: lbignum t (table_len * nLen) = Loops.repeati (j - 1) (bn_mod_precomp_table_mont_f n mu aM table_len) t01 in
-  //   let t4: lseq nat table_len = Loops.repeati (j - 1) (E.mod_precomp_table_mont_f (bits t) nLen (bn_v n) (v mu) (bn_v aM) table_len) t02 in
+  if j = 0 then begin
+    Loops.eq_repeati0 j (bn_mod_precomp_table_mont_f n mu aM table_len) t01;
+    Loops.eq_repeati0 j (E.mod_precomp_table_mont_f (bits t) nLen (bn_v n) (v mu) (bn_v aM) table_len) t02;
+    () end
+  else begin
+    let t3 = Loops.repeati (j - 1) (bn_mod_precomp_table_mont_f n mu aM table_len) t01 in
+    let t4 = Loops.repeati (j - 1) (E.mod_precomp_table_mont_f (bits t) nLen (bn_v n) (v mu) (bn_v aM) table_len) t02 in
+    bn_mod_precomp_table_mont_loop_lemma n mu table_len aM t01 t02 (j - 1);
+    //assert (forall (i:nat{i < j + 1}). {:pattern (bn_mod_precomp_table_mont_map n table_len t3 t4 i) }
+      //bn_mod_precomp_table_mont_map n table_len t3 t4 i);
 
-  //   Loops.unfold_repeati j (bn_mod_precomp_table_mont_f n mu aM table_len) t01 (j - 1);
-  //   Loops.unfold_repeati j (E.mod_precomp_table_mont_f (bits t) nLen (bn_v n) (v mu) (bn_v aM) table_len) t02 (j - 1);
-  //   bn_mod_precomp_table_mont_loop_lemma n mu table_len aM t01 t02 (j - 1);
+    Loops.unfold_repeati j (bn_mod_precomp_table_mont_f n mu aM table_len) t01 (j - 1);
+    //assert (t1 == bn_mod_precomp_table_mont_f n mu aM table_len (j - 1) t3);
+    Loops.unfold_repeati j (E.mod_precomp_table_mont_f (bits t) nLen (bn_v n) (v mu) (bn_v aM) table_len) t02 (j - 1);
+    //assert (t2 == E.mod_precomp_table_mont_f (bits t) nLen (bn_v n) (v mu) (bn_v aM) table_len (j - 1) t4);
 
-  //   // assert (forall (i:nat{i < j + 1}).
-  //   //  (Math.Lemmas.lemma_mult_le_right nLen (i + 1) (table_len);
-  //   //   assert (i * nLen + nLen <= table_len * nLen);
-  //   //   let bi = sub t3 (i * nLen) nLen in bn_v bi == index t4 i));
-
-  //   // assert (index t2 (j + 1) == M.mont_mul (bits t) nLen (bn_v n) (v mu) t4.[j] (bn_v aM));
-
-  //   assume (forall (i:nat{i < j + 2}).
-  //    (Math.Lemmas.lemma_mult_le_right nLen (i + 1) (table_len);
-  //     assert (i * nLen + nLen <= table_len * nLen);
-  //     let bi = sub t1 (i * nLen) nLen in bn_v bi == index t2 i));
-  //   () end
+    bn_mod_precomp_table_mont_step_lemma #t #nLen n mu aM table_len (j - 1) t3 t4;
+    //assert (forall (i:nat{i < j + 2}). {:pattern bn_mod_precomp_table_mont_map n table_len t1 t2 i}
+      //bn_mod_precomp_table_mont_map n table_len t1 t2 i);
+    () end
 
 
 val bn_mod_precomp_table_mont_lemma:
@@ -278,14 +384,11 @@ val bn_mod_precomp_table_mont_lemma:
   -> i:nat{i < table_len} -> Lemma
   (requires
     BM.bn_mont_pre n mu /\ bn_v aM < bn_v n /\
-    bn_v oneM == M.to_mont (bits t) nLen (bn_v n) (v mu) 1)
+    bn_v oneM == M.mont_one (bits t) nLen (bn_v n) (v mu) /\ bn_v oneM < bn_v n)
   (ensures
    (let t1 : lbignum t (table_len * nLen) = bn_mod_precomp_table_mont n mu table_len aM oneM in
     let t2 : lseq nat table_len = E.mod_precomp_table_mont (bits t) nLen (bn_v n) (v mu) table_len (bn_v aM) in
-    Math.Lemmas.lemma_mult_le_right nLen (i + 1) (table_len);
-    assert (i * nLen + nLen <= table_len * nLen);
-    let bi = sub t1 (i * nLen) nLen in
-    bn_v bi == index t2 i /\ bn_v bi < bn_v n))
+    bn_mod_precomp_table_mont_map n table_len t1 t2 i))
 
 let bn_mod_precomp_table_mont_lemma #t #nLen n mu table_len aM oneM i =
   let t01 = create (table_len * nLen) (uint #t 0) in
@@ -298,21 +401,64 @@ let bn_mod_precomp_table_mont_lemma #t #nLen n mu table_len aM oneM i =
   LSeq.eq_intro (sub t01 0 nLen) (sub t01' 0 nLen);
   assert (index t02 0 == bn_v (sub t01 0 nLen));
   assert (index t02 1 == bn_v (sub t01 nLen nLen));
-  bn_mod_precomp_table_mont_loop_lemma n mu table_len aM t01 t02 (table_len - 2);
+  bn_mod_precomp_table_mont_loop_lemma n mu table_len aM t01 t02 (table_len - 2)
 
-  let t1 : lbignum t (table_len * nLen) = bn_mod_precomp_table_mont n mu table_len aM oneM in
-  let t2 : lseq nat table_len = E.mod_precomp_table_mont (bits t) nLen (bn_v n) (v mu) table_len (bn_v aM) in
 
-  Math.Lemmas.lemma_mult_le_right nLen (i + 1) (table_len);
-  assert (i * nLen + nLen <= table_len * nLen);
-  let bi = sub t1 (i * nLen) nLen in
-  assert (bn_v bi == index t2 i);
+val table_select_ct_f_lemma:
+    #t:limb_t
+  -> #nLen:size_pos
+  -> table_len:size_nat{1 < table_len /\ table_len * nLen <= max_size_t}
+  -> table:lbignum t (table_len * nLen)
+  -> i:limb t{v i < table_len}
+  -> j:size_nat{j < table_len - 1}
+  -> acc:lbignum t nLen ->
+  Lemma (
+    let res = table_select_ct_f table_len table i j acc in
+    Math.Lemmas.lemma_mult_le_right nLen (j + 2) table_len;
+    let res_j = sub table ((j + 1) * nLen) nLen in
+    res == (if v i = j + 1 then res_j else acc))
 
-  bn_eval_bound n nLen;
-  M.mont_preconditions (bits t) nLen (bn_v n) (v mu);
-  assert (E.mont_pre (bits t) nLen (bn_v n) (v mu));
-  E.mod_precomp_table_mont_lemma (bits t) nLen (bn_v n) (v mu) table_len (bn_v aM) i;
-  assert (bn_v bi < bn_v n)
+let table_select_ct_f_lemma #t #nLen table_len table i j acc =
+  let c = eq_mask i (BB.size_to_limb (size (j + 1))) in
+  assert (v c == (if v i = j + 1 then ones_v t else 0));
+
+  Math.Lemmas.lemma_mult_le_right nLen (j + 2) table_len;
+  let res_j = sub table ((j + 1) * nLen) nLen in
+  let res = map2 (BB.mask_select c) res_j acc in
+  BB.lseq_mask_select_lemma res_j acc c
+
+
+val table_select_ct_loop_lemma:
+    #t:limb_t
+  -> #nLen:size_pos
+  -> table_len:size_nat{1 < table_len /\ table_len * nLen <= max_size_t}
+  -> table:lbignum t (table_len * nLen)
+  -> i:limb t{v i < table_len} ->
+  Pure (lbignum t nLen)
+  (requires True)
+  (ensures  fun res ->
+    let res0 : lbignum t nLen = sub table 0 nLen in
+    Math.Lemmas.lemma_mult_le_right nLen (v i + 1) table_len;
+    res == Loops.repeati (table_len - 1) (table_select_ct_f table_len table i) res0 /\
+    res == sub table (v i * nLen) nLen)
+
+let table_select_ct_loop_lemma #t #nLen table_len table i =
+  let res0 : lbignum t nLen = sub table 0 nLen in
+  Math.Lemmas.lemma_mult_le_right nLen (v i + 1) table_len;
+
+  Loops.eq_repeati0 (table_len - 1) (table_select_ct_f table_len table i) res0;
+  Loops.repeati_inductive (table_len - 1)
+  (fun j priv ->
+    priv == Loops.repeati j (table_select_ct_f table_len table i) res0 /\
+    priv == (if j >= v i then sub table (v i * nLen) nLen else res0))
+  (fun j priv ->
+    Loops.unfold_repeati (j + 1) (table_select_ct_f table_len table i) res0 j;
+    let res = table_select_ct_f table_len table i j priv in
+    table_select_ct_f_lemma table_len table i j priv;
+    Math.Lemmas.lemma_mult_le_right nLen (j + 2) table_len;
+    let res_j = sub table ((j + 1) * nLen) nLen in
+    assert (res == (if v i = j + 1 then res_j else priv));
+    res) res0
 
 
 val table_select_ct_lemma:
@@ -324,7 +470,27 @@ val table_select_ct_lemma:
   Lemma (Math.Lemmas.lemma_mult_le_right nLen (v i + 1) table_len;
     table_select_ct table_len table i == sub table (v i * nLen) nLen)
 
-let table_select_ct_lemma #t #nLen table_len table i = admit()
+let table_select_ct_lemma #t #nLen table_len table i =
+  let _ = table_select_ct_loop_lemma #t #nLen table_len table i in ()
+
+
+val bn_get_bits_l_lemma:
+    #t:limb_t
+  -> bBits:size_pos
+  -> bLen:size_nat{bLen == blocks bBits (bits t)}
+  -> b:lbignum t bLen
+  -> l:size_pos{l < bits t}
+  -> i:nat{i < bBits / l} -> Lemma
+  (requires bn_v b < pow2 bBits)
+  (ensures  v (bn_get_bits_l bBits bLen b l i) == LE.get_bits_l bBits (bn_v b) l i)
+
+let bn_get_bits_l_lemma #t bBits bLen b l i =
+  Math.Lemmas.lemma_mult_le_left l (i + 1) (bBits / l);
+  assert (l * (i + 1) <= l * (bBits / l));
+  Math.Lemmas.multiply_fractions bBits l;
+  assert (l * (i + 1) <= bBits);
+  let bits_l = BN.bn_get_bits b (bBits - l * i - l) l in
+  BN.bn_get_bits_lemma b (bBits - l * i - l) l
 
 
 val bn_mod_exp_fw_mont_f_lemma:
@@ -340,11 +506,11 @@ val bn_mod_exp_fw_mont_f_lemma:
   -> oneM:lbignum t nLen
   -> aM:lbignum t nLen
   -> accM:lbignum t nLen
-  -> i:nat{l * (i + 1) <= bBits} -> Lemma
+  -> i:nat{i < bBits / l} -> Lemma
   (requires
     BM.bn_mont_pre n mu /\ bn_v aM < bn_v n /\
     bn_v accM < bn_v n /\ bn_v b < pow2 bBits /\
-    bn_v oneM == M.to_mont (bits t) nLen (bn_v n) (v mu) 1)
+    bn_v oneM == M.mont_one (bits t) nLen (bn_v n) (v mu) /\ bn_v oneM < bn_v n)
   (ensures
    (let t1 = bn_mod_precomp_table_mont n mu table_len aM oneM in
     let t2 = E.mod_precomp_table_mont (bits t) nLen (bn_v n) (v mu) table_len (bn_v aM) in
@@ -357,13 +523,11 @@ let bn_mod_exp_fw_mont_f_lemma #t #nLen n mu bBits bLen b l table_len oneM aM ac
   let t1 = bn_mod_precomp_table_mont n mu table_len aM oneM in
   let t2 = E.mod_precomp_table_mont (bits t) nLen (bn_v n) (v mu) table_len (bn_v aM) in
 
-  let bits_l = BN.bn_get_bits b (bBits - l * i - l) l in
-  BN.bn_get_bits_lemma b (bBits - l * i - l) l;
-  assert (v bits_l == bn_v b / pow2 (bBits - l * i - l) % table_len);
+  let bits_l = bn_get_bits_l bBits bLen b l i in
+  bn_get_bits_l_lemma bBits bLen b l i;
   assert (v bits_l < table_len);
-  Math.Lemmas.lemma_mult_le_right nLen (v bits_l + 1) table_len;
-  assert (v bits_l * nLen + nLen <= table_len * nLen);
 
+  Math.Lemmas.lemma_mult_le_right nLen (v bits_l + 1) table_len;
   let a_powbits_l = sub t1 (v bits_l * nLen) nLen in
   bn_mod_precomp_table_mont_lemma n mu table_len aM oneM (v bits_l);
   assert (bn_v a_powbits_l < bn_v n);
@@ -392,7 +556,7 @@ val bn_mod_exp_fw_mont_rem_lemma:
   (requires
     BM.bn_mont_pre n mu /\ bn_v aM < bn_v n /\
     bn_v accM < bn_v n /\ bn_v b < pow2 bBits /\
-    bn_v oneM == M.to_mont (bits t) nLen (bn_v n) (v mu) 1)
+    bn_v oneM == M.mont_one (bits t) nLen (bn_v n) (v mu) /\ bn_v oneM < bn_v n)
   (ensures
    (let t1 = bn_mod_precomp_table_mont n mu table_len aM oneM in
     let t2 = E.mod_precomp_table_mont (bits t) nLen (bn_v n) (v mu) table_len (bn_v aM) in
@@ -418,8 +582,6 @@ let bn_mod_exp_fw_mont_rem_lemma #t #nLen n mu bBits bLen b l table_len oneM aM 
   assert (v bits_c < table_len);
 
   Math.Lemmas.lemma_mult_le_right nLen (v bits_c + 1) table_len;
-  assert (v bits_c * nLen + nLen <= table_len * nLen);
-
   let a_powbits_c = sub t1 (v bits_c * nLen) nLen in
   bn_mod_precomp_table_mont_lemma n mu table_len aM oneM (v bits_c);
   assert (bn_v a_powbits_c < bn_v n);
@@ -428,48 +590,46 @@ let bn_mod_exp_fw_mont_rem_lemma #t #nLen n mu bBits bLen b l table_len oneM aM 
   BM.bn_mont_mul_lemma n mu acc_pow2c a_powbits_c
 
 
-// val bn_mod_exp_fw_mont_loop_lemma:
-//     #t:limb_t
-//   -> #nLen:size_pos{nLen + nLen <= max_size_t}
-//   -> n:lbignum t nLen
-//   -> mu:limb t
-//   -> aM:lbignum t nLen
-//   -> bBits:size_pos
-//   -> b:lbignum t (blocks bBits (bits t))
-//   -> l:size_pos{l < bits t}
-//   -> table_len:size_nat{1 < table_len /\ table_len * nLen <= max_size_t /\ table_len == pow2 l}
-//   -> oneM:lbignum t nLen
-//   -> accM0:lbignum t nLen
-//   -> j:nat{l * j <= bBits} -> Lemma
-//   (requires
-//     BM.bn_mont_pre n mu /\ bn_v aM < bn_v n /\
-//     bn_v accM0 < bn_v n /\ bn_v b < pow2 bBits /\
-//     bn_v oneM == M.to_mont (bits t) nLen (bn_v n) (v mu) 1)
-//   (ensures
-//    (let t1 = bn_mod_precomp_table_mont n mu table_len aM oneM in
-//     let t2 = E.mod_precomp_table_mont (bits t) nLen (bn_v n) (v mu) table_len (bn_v aM) in
-//     let bLen = blocks bBits (bits t) in
+val bn_mod_exp_fw_mont_loop_lemma:
+    #t:limb_t
+  -> #nLen:size_pos{nLen + nLen <= max_size_t}
+  -> n:lbignum t nLen
+  -> mu:limb t
+  -> aM:lbignum t nLen
+  -> bBits:size_pos
+  -> b:lbignum t (blocks bBits (bits t))
+  -> l:size_pos{l < bits t}
+  -> table_len:size_nat{1 < table_len /\ table_len * nLen <= max_size_t /\ table_len == pow2 l}
+  -> oneM:lbignum t nLen
+  -> j:nat{j <= bBits / l} -> Lemma
+  (requires
+    BM.bn_mont_pre n mu /\ bn_v aM < bn_v n /\ bn_v b < pow2 bBits /\
+    bn_v oneM == M.mont_one (bits t) nLen (bn_v n) (v mu) /\ bn_v oneM < bn_v n)
+  (ensures
+   (let t1 = bn_mod_precomp_table_mont n mu table_len aM oneM in
+    let t2 = E.mod_precomp_table_mont (bits t) nLen (bn_v n) (v mu) table_len (bn_v aM) in
+    let bLen = blocks bBits (bits t) in
 
-//     let accM1: lbignum t nLen = Loops.repeati j (bn_mod_exp_fw_mont_f n mu bBits bLen b l table_len t1) accM0 in
-//     let accM2 = Loops.repeati j (E.mod_exp_fw_mont_f (bits t) nLen (bn_v n) (v mu) bBits (bn_v b) l table_len t2) (bn_v accM0) in
-//     bn_v accM1 == accM2 /\ bn_v accM1 < bn_v n))
+    let accM1 = Loops.repeati j (bn_mod_exp_fw_mont_f n mu bBits bLen b l table_len t1) oneM in
+    let accM2 = Loops.repeati j (E.mod_exp_fw_mont_f (bits t) nLen (bn_v n) (v mu) bBits (bn_v b) l table_len t2) (bn_v oneM) in
+    bn_v accM1 == accM2 /\ bn_v accM1 < bn_v n))
 
-// let rec bn_mod_exp_fw_mont_loop_lemma #t #nLen n mu aM bBits b l table_len oneM accM0 j =
-//   let t1 = bn_mod_precomp_table_mont n mu table_len aM oneM in
-//   let t2 = E.mod_precomp_table_mont (bits t) nLen (bn_v n) (v mu) table_len (bn_v aM) in
-//   let bLen = blocks bBits (bits t) in
+let rec bn_mod_exp_fw_mont_loop_lemma #t #nLen n mu aM bBits b l table_len oneM j =
+  let t1 = bn_mod_precomp_table_mont n mu table_len aM oneM in
+  let t2 = E.mod_precomp_table_mont (bits t) nLen (bn_v n) (v mu) table_len (bn_v aM) in
+  let bLen = blocks bBits (bits t) in
 
-//   if j = 0 then begin
-//     Loops.eq_repeati0 j (bn_mod_exp_fw_mont_f n mu bBits bLen b l table_len t1) accM0;
-//     Loops.eq_repeati0 j (E.mod_exp_fw_mont_f (bits t) nLen (bn_v n) (v mu) bBits (bn_v b) l table_len t2) (bn_v accM0) end
-//   else begin
-//     Math.Lemmas.lemma_mult_lt_left l (j - 1) j;
-//     let accM4 = Loops.repeati (j - 1) (bn_mod_exp_fw_mont_f n mu bBits bLen b l table_len t1) accM0 in
-//     Loops.unfold_repeati j (E.mod_exp_fw_mont_f (bits t) nLen (bn_v n) (v mu) bBits (bn_v b) l table_len t2) (bn_v accM0) (j - 1);
-//     Loops.unfold_repeati j (bn_mod_exp_fw_mont_f n mu bBits bLen b l table_len t1) accM0 (j - 1);
-//     bn_mod_exp_fw_mont_loop_lemma n mu aM bBits b l table_len oneM accM0 (j - 1);
-//     bn_mod_exp_fw_mont_f_lemma n mu bBits bLen b l table_len oneM aM accM4 (j - 1);
-//     () end
+  if j = 0 then begin
+    Loops.eq_repeati0 j (bn_mod_exp_fw_mont_f n mu bBits bLen b l table_len t1) oneM;
+    Loops.eq_repeati0 j (E.mod_exp_fw_mont_f (bits t) nLen (bn_v n) (v mu) bBits (bn_v b) l table_len t2) (bn_v oneM) end
+  else begin
+    let accM3 = Loops.repeati (j - 1) (bn_mod_exp_fw_mont_f n mu bBits bLen b l table_len t1) oneM in
+    let accM4 = Loops.repeati (j - 1) (E.mod_exp_fw_mont_f (bits t) nLen (bn_v n) (v mu) bBits (bn_v b) l table_len t2) (bn_v oneM) in
+    Loops.unfold_repeati j (E.mod_exp_fw_mont_f (bits t) nLen (bn_v n) (v mu) bBits (bn_v b) l table_len t2) (bn_v oneM) (j - 1);
+    Loops.unfold_repeati j (bn_mod_exp_fw_mont_f n mu bBits bLen b l table_len t1) oneM (j - 1);
+    bn_mod_exp_fw_mont_loop_lemma n mu aM bBits b l table_len oneM (j - 1);
+    bn_mod_exp_fw_mont_f_lemma #t #nLen n mu bBits bLen b l table_len oneM aM accM3 (j - 1);
+    () end
 
 
 val bn_mod_exp_fw_mont_aux_lemma:
@@ -500,10 +660,9 @@ let bn_mod_exp_fw_mont_aux_lemma #t #nLen n mu aM bBits b l r2 =
 
   let table = bn_mod_precomp_table_mont n mu table_len aM oneM in
   Math.Lemmas.multiply_fractions bBits l;
-  let accM: lbignum t nLen = Loops.repeati (bBits / l) (bn_mod_exp_fw_mont_f n mu bBits bLen b l table_len table) oneM in
-  admit();
-  //bn_mod_exp_fw_mont_loop_lemma n mu aM bBits b l table_len oneM oneM (bBits / l);
-  //let res = if bBits % l = 0 then accM else bn_mod_exp_fw_mont_rem n mu bBits bLen b l table_len table accM in
+  let accM = Loops.repeati (bBits / l) (bn_mod_exp_fw_mont_f n mu bBits bLen b l table_len table) oneM in
+
+  bn_mod_exp_fw_mont_loop_lemma n mu aM bBits b l table_len oneM (bBits / l);
   if bBits % l = 0 then ()
   else bn_mod_exp_fw_mont_rem_lemma n mu bBits bLen b l table_len oneM aM accM
 
